theories/approxis/examples/advantage.v
@@ -1,0 +1,29 @@
+From clutch.approxis Require Import approxis.
+From clutch.approxis Require Export bounded_oracle.
+From Coquelicot Require Import Lub.
+Set Default Proof Using "Type*".
+
+
+Definition pr_dist (A : val) (G G' : expr)
+  (σ σ' : state) (v : val) :=
+  Rabs ( (( lim_exec (A G, σ)) v) - (lim_exec (A G', σ') v) )%R.
+
+Definition advantage (A : val) (G G' : expr) :=
+  Lub_Rbar (λ ε : R, ∃ (σ σ' : state) (v : val), pr_dist A G G' σ σ' v = ε)%R.
+
+Lemma advantage_uniform (A : val) (G G' : expr) (ε : R) :
+  (∀ (σ σ' : state) (v : val), pr_dist A G G' σ σ' v <= ε)%R ->
+  (Rbar.Rbar_le (advantage A G G') (Rbar.Finite ε)).
+Proof.
+  intros hε.
+  rewrite /advantage.
+  set (E := (λ ε0 : R, ∃ (σ σ' : state) (v : val), pr_dist A G G' σ σ' v = ε0)).
+  opose proof (Lub_Rbar_correct E) as h.
+  rewrite /is_lub_Rbar in h.
+  destruct h as [h1 h2].
+  apply h2.
+  rewrite /is_ub_Rbar.
+  intros ε' (σ & σ' & v & hε').
+  apply rbar_le_rle.
+  rewrite -hε'. apply hε.
+Qed.
