theories/approxis/examples/security_aux.v
@@ -1,0 +1,21 @@
+From clutch.approxis Require Import approxis map list.
+(* From clutch.approxis.examples Require Import prf symmetric prf_cpa. *)
+Set Default Proof Using "Type*".
+
+Definition TOption (T : type) : type := (TUnit + T)%ty.
+
+Definition opt_mult : val :=
+  λ:"opt",
+    match: "opt" with
+    | NONE => NONE
+    | SOME "vopt" =>
+        match: "vopt" with
+        | NONE => NONE
+        | SOME "v" => SOME "v"
+        end
+    end.
+
+Fact opt_mult_typed (A : type) : (⊢ᵥ opt_mult : (TOption (TOption A) → TOption A)%ty).
+Proof.
+  rewrite /opt_mult. tychk.
+Qed.
